root verified

examples/algorithms/Uf.fst
@@ -3,6 +3,7 @@ module Uf
 open FStar.Heap
 open FStar.List.Tot
 open FStar.Squash
+open FStar.Classical
 open FStar.Ghost
 open FStar.ST
 open FStar.TSet
@@ -10,12 +11,11 @@ open FStar.TSet
 
 type uf (a : Type) : Type = { content:a ; parent:ref (option (uf a)) }
 
+noeq type reachable (#a:eqtype) (h:heap) (x:uf a) : uf a -> Type =
+| Immediately : y:(uf a){sel h y.parent = Some x} -> reachable h x y
+| Later : y:(uf a) -> reachable h x y -> z:(uf a){sel h z.parent = Some y} -> reachable h x z
 
-noeq type reachable (#a:eqtype) (h:heap) : uf a -> uf a -> Type =
-| Immediately : x:uf a -> y:(uf a){sel h y.parent = Some x} -> reachable h x y
-| Later : x:uf a -> y:(uf a) -> reachable h x y -> z:(uf a){sel h z.parent = Some y} -> reachable h x z
-
-
+(*
 val give_witness : #p:Type -> p -> Pure unit (requires True) (ensures (fun _ -> p))
 let give_witness #p x = give_proof (return_squash x)
 
@@ -31,7 +31,7 @@ let intro_forall #a #p f =
 
 val give_proof0 : #p:Type0 -> p -> Pure unit (requires True) (ensures (fun _ -> p))
 let give_proof0 #p _ = ()
-
+*)
 
 noeq type funcaccessible (#a:Type0) (f: a -> GTot (option a)) (u : a) : Type0 =
 | FAcc : next:(match f u with | Some v -> funcaccessible f v | None -> unit) -> funcaccessible f u
@@ -47,32 +47,37 @@ assume val recall_step : #a:eqtype -> h:heap -> z:uf a -> y:uf a -> Lemma (requi
 
 let rec recall_reachable (#a:eqtype) (h:heap) (u1:uf a) (u2:uf a) (w:reachable h u1 u2) : Lemma (requires (Heap.contains h u2.parent)) (ensures (Heap.contains h u1.parent)) (decreases w) =
   match w with
-  | Immediately y z -> recall_step h z y
-  | Later x y w0 z -> recall_step h z y ; recall_reachable h x y w0
+  | Immediately z -> recall_step h z u1
+  | Later y w0 z -> recall_step h z y ; recall_reachable h u1 y w0
 
 
 let rec pullback_reachable (#a:eqtype) (h0:heap) (h1:heap) (u1:uf a) (u2: uf a) (w:reachable h1 u1 u2) : Pure (reachable h0 u1 u2) (requires (modifies_none h0 h1 /\ Heap.contains h0 u2.parent)) (ensures (fun _ -> True)) (decreases w) =
   match w with
-  | Immediately y z -> Immediately y z
-  | Later x y w0 z -> recall_step h0 z y ; Later x y (pullback_reachable h0 h1 x y w0) z
+  | Immediately z -> Immediately z
+  | Later y w0 z -> recall_step h0 z y ; Later y (pullback_reachable h0 h1 u1 y w0) z
 
 
 let rec pushforward_reachable (#a:eqtype) (h0:heap) (h1:heap) (u1:uf a) (u2: uf a) (w:reachable h0 u1 u2) : Pure (reachable h1 u1 u2) (requires (modifies_none h0 h1 /\ Heap.contains h0 u2.parent)) (ensures (fun _ -> True)) (decreases w) =
     match w with
-    | Immediately y z -> Immediately y z
-    | Later x y w0 z -> recall_step h0 z y ; Later x y (pushforward_reachable h0 h1 x y w0) z
+    | Immediately z -> Immediately z
+    | Later y w0 z -> recall_step h0 z y ; Later y (pushforward_reachable h0 h1 u1 y w0) z
 
 //assume val recall_reachable : #a:eqtype -> h:heap -> u1:(uf a) -> u2:(uf a) -> Lemma (Heap.contains h u1.parent /\ reachable h u2 u1 ==> Heap.contains h u2.parent)
 //assume val pullback_reachable : #a:eqtype -> h0:heap -> h1:heap -> u1:(uf a) -> u2:(uf a) -> reachable h1 u1 u2 -> Pure (reachable h0 u1 u2) (requires (modifies_none h0 h1 /\ Heap.contains h0 u2.parent)) (ensures (fun _ -> True))
 
 
-let uf_invariant (a:eqtype) (h:heap) : Type0 = u0:(ufh a h) -> GTot ((funcaccessible (reach a h) u0) * (u1: uf a -> reachable h u1 u0 -> Lemma (u1.parent <> u0.parent)))
+let uf_invariant (a:eqtype) (h:heap) : Type0 = (forall (u0:ufh a h). funcaccessible (reach a h) u0) ///\ (forall (u0: ufh a h) (u1: ufh a h). u0.parent = u1.parent ==> u0 = u1) // * (u1: uf a -> reachable h u1 u0 -> Lemma (u1.parent <> u0.parent)))
+let uf_invariant_fun (#a:eqtype) (h:heap) : Tot Type0 = (u0:ufh a h) -> GTot (funcaccessible (reach a h) u0)
 
+let maintain_uf_invariant (a:eqtype) (h0:heap) (h1:heap) ($f : uf_invariant_fun h0 -> GTot (uf_invariant_fun h1)) : Lemma (requires (uf_invariant a h0)) (ensures (uf_invariant a h1)) =
+  give_proof #(uf_invariant a h1) (map_squash (get_proof (uf_invariant a h0)) (fun (sq_uf_inv0 : squash (uf_invariant_fun h0)) -> map_squash sq_uf_inv0 f))
+
+assume val uf_invariant_termination : (a:eqtype) -> (h:heap) -> (u:ufh a h) -> (p:ufh a h) -> Lemma (requires (uf_invariant a h /\ sel h u.parent = Some p)) (ensures (p << u))
 
 //let typeof (a:Type) ($f : a) = f
 
 
-assume val axiom1_dep2 : #a:Type -> #b:(a->Type) -> #c:(x:a -> y:b x -> Type) -> f:(x:a -> y:b x -> Tot (c x y)) -> x:a -> y: b x -> Lemma (f x y << f)
+//assume val axiom1_dep2 : #a:Type -> #b:(a->Type) -> #c:(x:a -> y:b x -> Type) -> f:(x:a -> y:b x -> Tot (c x y)) -> x:a -> y: b x -> Lemma (f x y << f)
 
 //let pullback_contains (#a:Type) (h0:heap) (h1:heap) (x:ref a) (r0:ref a) : Lemma (requires (exists v. h1 == upd h0 r0 v /\ Heap.contains h1 x /\ x <> r0)) (ensures (Heap.contains h0 x)) = ()
 
@@ -86,24 +91,16 @@ let make_uf (#a:eqtype) (x:a) : ST (uf a) (requires (uf_invariant a)) (ensures (
   let h0 = get () in
   let res : uf a = { content = x ; parent = alloc None } in
   let h1 = get () in
-  let aux (uf_inv:uf_invariant a h0) : GTot (squash (uf_invariant a h1)) =
+  let uf_inv1 (uf_inv0:uf_invariant_fun h0) (u: ufh a h1) : GTot (funcaccessible (reach a h1) u) =
     let rec pushforward_accessible (u:ufh a h1) (acc0 : funcaccessible (reach a h0) u) : GTot (funcaccessible (reach a h1) u) (decreases acc0) =
       match reach a h1 u with | None -> FAcc () | Some v -> recall_step h1 u v ; FAcc (pushforward_accessible v acc0.next)
-    in
-    let wf (u1 : ufh a h1) : GTot (funcaccessible (reach a h1) u1) =
-      if u1.parent = res.parent then FAcc () else let u1 : uf a = u1 in pushforward_accessible u1 (fst (uf_inv u1))
-    in
-    let antialiasing (u0:ufh a h1) (u1:uf a) (w:reachable h1 u1 u0) : Lemma (u0.parent <> u1.parent) =
-      if u0.parent = res.parent
-      then begin match w with end
-      else begin let u0 : uf a = u0 in (snd (uf_inv u0)) u1 (pullback_reachable h0 h1 u1 u0 w) end
-    in
-    return_squash begin fun u0 -> (wf u0, antialiasing u0) end
-  in
-  give_proof (bind_squash (get_proof (uf_invariant a h0)) aux) ;
+    in if u.parent = res.parent then FAcc () else let u : uf a = u in pushforward_accessible u (uf_inv0 u)
+  in maintain_uf_invariant a h0 h1 uf_inv1 ;
   res
 
 
+
+(*
 let intro_forall_impl (#a:Type) (#b:a -> Type0) (#c:a -> Type0) ($f:x:a -> b x -> Lemma (c x)) : Lemma (forall (x:a). b x ==> c x) =
   let f0 (x:a) (y:b x) : GTot (squash (c x)) = f x y ; get_proof (c x) in
   let f1 (x:a) : GTot (squash (squash (b x -> GTot (c x)))) = return_squash (squash_double_arrow (return_squash (f0 x))) in
@@ -111,16 +108,25 @@ let intro_forall_impl (#a:Type) (#b:a -> Type0) (#c:a -> Type0) ($f:x:a -> b x -
   let f3 : squash (x:a -> GTot (b x ==> c x)) = f2 in
   let res : (forall (x:a). b x ==> c x) = f3 in
   give_witness res
+  *)
 
-
-let rec collect_above (#a:eqtype) (h:heap) (u : uf a) (w:funcaccessible (reach a h) u) : Ghost (set aref) (requires True) (ensures (fun s -> forall v. (sel h v.parent <> None /\ (v = u \/ reachable h v u)) <==> mem (Ref v.parent) s)) (decreases w) =
+(*
+let rec collect_above (#a:eqtype) (h:heap) (u : ufh a h) : Ghost (set aref) (requires (uf_invariant a h)) (ensures (fun s -> forall v. (sel h v.parent <> None /\ (v = u \/ reachable h v u)) <==> mem (Ref v.parent) s)) (decreases u) =
   match sel h u.parent with
-    | None -> let f (v:uf a) : Tot ((reachable h v u) ==> False) = intro_impl (fun w -> match w with) in give_witness (intro_forall f) ; assert (forall v. ~(reachable h v u)) ; empty
+    | None ->
+      let f (v:uf a) : GTot ((reachable h v u) ==> False) = impl_intro_gtot (let g (w:reachable h v u) : GTot False = match w with in g) in
+      give_witness (forall_intro_gtot f) ;
+      assert (forall v. ~(reachable h v u)) ;
+      empty
     | Some p ->
-      let f (v:uf a) (w:reachable h v u): Lemma (v.parent = p.parent \/ reachable h v p) = match w with | Immediately _ _ -> () | Later _ _ w0 _ -> give_witness w0 in
-      intro_forall_impl f ; assert(forall (v:uf a). (reachable h v u ==> (v.parent = p.parent \/ reachable h v p)))  ;
-      recall_step h u p ; admit () ; singleton (Ref u.parent) `union` collect_above h p w.next
+      let f (v:uf a) (w:reachable h v u): Lemma (v.parent = p.parent \/ reachable h v p) = match w with | Immediately _ -> () | Later _ w0 _ -> give_witness w0 in
+      forall_intro (let g (v:uf a) : Lemma (reachable h v u ==> v.parent = p.parent \/ reachable h v p) = impl_intro (f v) in g) ;
+      assert(forall (v:uf a). (reachable h v u ==> (v.parent = p.parent \/ reachable h v p)))  ;
+      recall_step h u p ; uf_invariant_termination a h u p ; admit () ; singleton (Ref u.parent) `union` collect_above h p
+*)
 
+
+let distinct_cell_lemma (#a:eqtype) (h:heap) (r1:ref a) (r2: ref a) : Lemma (sel h r1 <> sel h r2 ==> r1 <> r2) = ()
 
 (* Without invariants :
 
@@ -133,14 +139,37 @@ let rec collect_above (#a:eqtype) (h:heap) (u : uf a) (w:funcaccessible (reach a
       r
 *)
 
-let rec root (#a:eqtype) (u:uf a) : ST (uf a) (requires (uf_invariant a)) (ensures (fun h0 r h1 -> modifies (collect_above h0 u (admit ())) h0 h1 /\ uf_invariant a h1 /\ (r = u \/ reachable h0 r u) /\ sel h1 r.parent = None)) =
+let rec root (#a:eqtype) (u:uf a) : ST (uf a) (requires (uf_invariant a)) (ensures (fun h0 r h1 -> (* Heap.contains h0 u.parent /\ uf_invariant a h0 /\ modifies (collect_above h0 u) h0 h1 /\*) uf_invariant a h1 /\ (r = u \/ reachable h0 r u) /\ sel h0 r.parent = None /\ sel h1 r.parent = None)) (decreases u) (* WARNING : check the decrease clause by hand for now *) =
   match !u.parent with
-  | None -> u
+  | None -> admit () ; u
   | Some p ->
     let h0 = get () in
+    recall u.parent ;
+    recall p.parent ;
+    uf_invariant_termination a h0 u p ;
+    assert ( p << u ) ;
     let r = root p in
     let h1 = get () in
-    let sqw0 : squash (reachable h0 r u) =
+    assert (sel h0 u.parent = Some p) ;
+    distinct_cell_lemma h0 r.parent u.parent ;
+    assert (r.parent <> u.parent) ;
+    recall u.parent ;
+    u.parent := Some r ;
+    let h2 = get () in
+    assert (forall (u0 : ufh a h2). Heap.contains h1 u0.parent);
+    assert (forall (u0 : ufh a h2). u0.parent <> u.parent ==> reach a h2 u0 = reach a h1 u0);
+    let uf_inv2 (uf_inv1: uf_invariant_fun h1) (u1:ufh a h2) : GTot (funcaccessible (reach a h2) u1) =
+      let rec pushforward (u0:ufh a h1) (w : funcaccessible (reach a h1) u0) : GTot (funcaccessible (reach a h2) u0) (decreases w) =
+        if u0.parent = u.parent
+        then ( match reach a h2 u0 with | Some r0 -> let wr0 : funcaccessible (reach a h2) r0 = match reach a h2 r0 with | None -> FAcc () in FAcc wr0 ) (* TODO : Something's wrong here FAcc (FAcc ()) should be enough  *)
+        else match reach a h2 u0 with | None -> FAcc () | Some v -> recall_step h1 u0 v ; FAcc (pushforward v w.next)
+      in let u1 : uf a = u1 in pushforward u1 (uf_inv1 u1)
+    in maintain_uf_invariant a h1 h2 uf_inv2 ;
+    assert (uf_invariant a h2) ;
+    if p = r then give_witness #(reachable h0 r u) (Immediately u) else give_proof (map_squash (get_proof (reachable h0 r p)) (fun w -> Later p w u)) ;
+    assert (reachable h0 r u) ;
+    //admit () ;
+    (*let sqw0 : squash (reachable h0 r u) =
       let res = if r = p then return_squash (Immediately p u) else map_squash (get_proof (reachable h0 r p)) (fun w -> Later r p w u) in
       admit () ; res
     in
@@ -148,8 +177,6 @@ let rec root (#a:eqtype) (u:uf a) : ST (uf a) (requires (uf_invariant a)) (ensur
     assert (u.parent <> r.parent) ;
     assert (u <> r) ;
     assert (sel h1 r.parent = None) ;
-    u.parent := Some r ;
-    let h2 = get () in
     let aux (uf_inv: uf_invariant a h1) : GTot (squash (uf_invariant a h2)) =
       let wf (u1:ufh a h2) : GTot (funcaccessible (reach a h2) u1) =
         let root_accessible : funcaccessible (reach a h2) r = FAcc () in
@@ -167,7 +194,7 @@ let rec root (#a:eqtype) (u:uf a) : ST (uf a) (requires (uf_invariant a)) (ensur
     in
     give_proof (bind_squash (get_proof (uf_invariant a h1)) aux) ;
    assert (uf_invariant a h2) ;
-  assert (sel h2 r.parent = None) ;
+  assert (sel h2 r.parent = None) ;*)
     r
 
 
